WIP; wpsim_coind completed

simulations/wpsim/wpsim.v
@@ -5,11 +5,12 @@ Require Export invariants.
 
 From stdpp Require Import coPset.
 Section wpsim.
-  (* Context `{@SRFIntp.t (domain Σ) α, Γ : HRA, !subG Γ Σ, !invGS Σ Γ}. *)
   Context `{!sinvGS Σ Γ α β τ}.
   Context {fl_s fl_t : alist string (Any.t → itree hmodE Any.t)}.
   Context {Ist : nat → alist key Any.t → alist key Any.t → iProp Σ}.
   Context {my_tid : nat}.
+  Context {u : univ_id}.
+  Context {n : level}.
 
   Local Definition state : Type := alist key Any.t.
   Local Definition post (R : Type) : Type := nat → state * R → state * R → iProp Σ.
@@ -19,16 +20,20 @@ Section wpsim.
   Implicit Types r g : rel.
   Implicit Types ps pt : bool.
   Implicit Types nths : nat.
-  Implicit Types u : univ_id.
-  Implicit Types n : level.
   Implicit Types E : coPset.
 
   (* TODO : abstraction into mixins *)
-  Local Definition wpsim_pre u n E : iProp Σ := own_admin ∗ univs u n ∗ wsats u n E.
+  (* TODO : hard-code nodup conditions *)
+  Local Definition wpsim_pre E : iProp Σ := own_admin ∗ univs u n ∗ wsats u n E.
+  Local Definition wpsim_rel (r : rel) : rel :=
+    λ R RR ps pt nths '(st_s, i_s) '(st_t, i_t),
+      (wpsim_pre ⊤ ∗ r R RR ps pt nths (st_s, i_s) (st_t, i_t))%I.
+
   (* Simulation relation that corresponds to iris' weakest precondition *)
   (* TODO : seal *)
-  Local Definition wpsim_def r g R RR ps pt nths st_s st_t u n E : iProp Σ :=
-    wpsim_pre u n E -∗ @isim Σ fl_s fl_t Ist my_tid false r g R RR ps pt nths st_s st_t.
+  Local Definition wpsim_def r g R RR ps pt nths st_s st_t E : iProp Σ :=
+    wpsim_pre E -∗
+    @isim Σ fl_s fl_t Ist my_tid false (wpsim_rel r) (wpsim_rel g) R RR ps pt nths st_s st_t.
   Local Definition wpsim_aux : seal (@wpsim_def). Proof. by eexists. Qed.
   Definition wpsim := wpsim_aux.(unseal).
   Local Definition wpsim_eq : @wpsim = @wpsim_def := wpsim_aux.(seal_eq).
@@ -36,127 +41,194 @@ Section wpsim.
 
   (* Primitive simulation rules *)
   (* Mostly will not be used *)
-  Lemma wpsim_ret r g R RR ps pt nths st_s st_t rs rt u n E :
-    RR nths (st_s, rs) (st_t, rt) ⊢ wpsim r g R RR ps pt nths (st_s, Ret rs) (st_t, Ret rt) u n ⊤.
+  Lemma wpsim_ret r g R RR ps pt nths st_s st_t rs rt E :
+    RR nths (st_s, rs) (st_t, rt) ⊢ wpsim r g R RR ps pt nths (st_s, Ret rs) (st_t, Ret rt) ⊤.
   Proof. unseal; iIntros "RR I". iApply isim_ret; done. Qed.
 
-  Lemma wpim_call r g R RR ps pt nths st_s st_t fn arg k_s k_t u n E :
+  Lemma wpim_call r g R RR ps pt nths st_s st_t fn arg k_s k_t E :
     Ist nths st_s st_t ∗
     (∀ ret nths' st_s' st_t'
       (NODS : List.NoDup (List.map fst st_s'))
       (NODD : List.NoDup (List.map fst st_t')),
       Ist nths' st_s' st_t' -∗
-      wpsim r g R RR true true nths' (st_s', k_s ret) (st_t', k_t ret) u n E) ⊢
+      wpsim r g R RR true true nths' (st_s', k_s ret) (st_t', k_t ret) E) ⊢
     wpsim r g R RR ps pt nths
-      (st_s, trigger (Call fn arg) >>= k_s) (st_t, trigger (Call fn arg) >>= k_t) u n E.
+      (st_s, trigger (Call fn arg) >>= k_s) (st_t, trigger (Call fn arg) >>= k_t) E.
   Proof.
     unseal; iIntros "[IST CONT] I".
     rewrite -isim_call; iFrame.
     iIntros (??????) "IST !>"; iApply ("CONT" with "[] [] [IST]"); iFrame; try iPureIntro; ss.
   Qed.
 
-  Lemma wpsim_io r g R RR ps pt nths st_s st_t fn I O (arg : I) k_s k_t u n E :
-    (∀ (ret : O), wpsim r g R RR true true nths (st_s, k_s ret) (st_t, k_t ret) u n E) ⊢
+  Lemma wpsim_io r g R RR ps pt nths st_s st_t fn I O (arg : I) k_s k_t E :
+    (∀ (ret : O), wpsim r g R RR true true nths (st_s, k_s ret) (st_t, k_t ret) E) ⊢
     wpsim r g R RR ps pt nths
       (st_s, trigger (IO fn arg) >>= k_s)
-      (st_t, trigger (IO fn arg) >>= k_t) u n E.
+      (st_t, trigger (IO fn arg) >>= k_t) E.
   Proof. unseal; iIntros "RR I". iApply isim_io. iIntros (ret); iApply "RR"; iFrame. Qed.
 
-  Lemma wpsim_tau_src r g R RR ps pt nths st_s st_t i_s i_t u n E :
-    wpsim r g R RR true pt nths (st_s, i_s) (st_t, i_t) u n E ⊢
-    wpsim r g R RR ps pt nths (st_s, tau;; i_s) (st_t, i_t) u n E.
+  Lemma wpsim_tau_src r g R RR ps pt nths st_s st_t i_s i_t E :
+    wpsim r g R RR true pt nths (st_s, i_s) (st_t, i_t) E ⊢
+    wpsim r g R RR ps pt nths (st_s, tau;; i_s) (st_t, i_t) E.
   Proof. unseal; iIntros "RR I". iApply isim_tau_src; iApply "RR"; iFrame. Qed.
 
-  Lemma wpsim_tau_tgt r g R RR ps pt nths st_s st_t i_s i_t u n E :
-    wpsim r g R RR ps true nths (st_s, i_s) (st_t, i_t) u n E ⊢
-    wpsim r g R RR ps pt nths (st_s, i_s) (st_t, tau;; i_t) u n E.
+  Lemma wpsim_tau_tgt r g R RR ps pt nths st_s st_t i_s i_t E :
+    wpsim r g R RR ps true nths (st_s, i_s) (st_t, i_t) E ⊢
+    wpsim r g R RR ps pt nths (st_s, i_s) (st_t, tau;; i_t) E.
   Proof. unseal; iIntros "RR I". iApply isim_tau_tgt; iApply "RR"; iFrame. Qed.
 
-  Lemma wpsim_inline_src r g R RR ps pt nths st_s st_t fn arg f_s k_s i_t u n E :
+  Lemma wpsim_inline_src r g R RR ps pt nths st_s st_t fn arg f_s k_s i_t E :
     alist_find fn fl_s = Some f_s →
     wpsim r g R RR true pt nths
       (st_s, x <- (ret <- (f_s arg);; (tau;; tau;; Ret ret));; (k_s x))
-      (st_t, i_t) u n E ⊢
-    wpsim r g R RR ps pt nths (st_s, trigger (Call fn arg) >>= k_s) (st_t, i_t) u n E.
+      (st_t, i_t) E ⊢
+    wpsim r g R RR ps pt nths (st_s, trigger (Call fn arg) >>= k_s) (st_t, i_t) E.
   Proof. i; unseal; iIntros "RR I". iApply isim_inline_src; eauto. iApply "RR"; iFrame. Qed.
 
-  Lemma wpsim_inline_tgt r g R RR ps pt nths st_s st_t fn arg i_s f_t k_t u n E :
+  Lemma wpsim_inline_tgt r g R RR ps pt nths st_s st_t fn arg i_s f_t k_t E :
     alist_find fn fl_t = Some f_t →
     wpsim r g R RR ps true nths
       (st_s, i_s)
-      (st_t, x <- (ret <- (f_t arg);; (tau;; tau;; Ret ret));; (k_t x)) u n E ⊢
-    wpsim r g R RR ps pt nths (st_s, i_s) (st_t, trigger (Call fn arg) >>= k_t) u n E.
+      (st_t, x <- (ret <- (f_t arg);; (tau;; tau;; Ret ret));; (k_t x)) E ⊢
+    wpsim r g R RR ps pt nths (st_s, i_s) (st_t, trigger (Call fn arg) >>= k_t) E.
   Proof. i; unseal; iIntros "RR I". iApply isim_inline_tgt; eauto. iApply "RR"; iFrame. Qed.
 
-  Lemma wpsim_take_src X r g R RR ps pt nths st_s st_t k_s i_t u n E :
-    (∀ x, wpsim r g R RR true pt nths (st_s, k_s x) (st_t, i_t) u n E) ⊢
-    wpsim r g R RR ps pt nths (st_s, trigger (Take X) >>= k_s) (st_t, i_t) u n E.
+  Lemma wpsim_take_src X r g R RR ps pt nths st_s st_t k_s i_t E :
+    (∀ x, wpsim r g R RR true pt nths (st_s, k_s x) (st_t, i_t) E) ⊢
+    wpsim r g R RR ps pt nths (st_s, trigger (Take X) >>= k_s) (st_t, i_t) E.
   Proof.
     unseal; iIntros "RR I". iApply isim_take_src; eauto. iIntros (x); iApply "RR"; iFrame.
   Qed.
 
-  Lemma wpsim_take_tgt X r g R RR ps pt nths st_s st_t i_s k_t u n E :
-    (∃ x, wpsim r g R RR ps true nths (st_s, i_s) (st_t, k_t x) u n E) ⊢
-    wpsim r g R RR ps pt nths (st_s, i_s) (st_t, trigger (Take X) >>= k_t) u n E.
+  Lemma wpsim_take_tgt X r g R RR ps pt nths st_s st_t i_s k_t E :
+    (∃ x, wpsim r g R RR ps true nths (st_s, i_s) (st_t, k_t x) E) ⊢
+    wpsim r g R RR ps pt nths (st_s, i_s) (st_t, trigger (Take X) >>= k_t) E.
   Proof.
     unseal; iIntros "[%x RR] I". iApply isim_take_tgt; eauto. iExists _; iApply "RR"; iFrame.
   Qed.
 
-  Lemma wpsim_choose_src X r g R RR ps pt nths st_s st_t k_s i_t u n E :
-    (∃ x, wpsim r g R RR true pt nths (st_s, k_s x) (st_t, i_t) u n E) ⊢
-    wpsim r g R RR ps pt nths (st_s, trigger (Choose X) >>= k_s) (st_t, i_t) u n E.
+  Lemma wpsim_choose_src X r g R RR ps pt nths st_s st_t k_s i_t E :
+    (∃ x, wpsim r g R RR true pt nths (st_s, k_s x) (st_t, i_t) E) ⊢
+    wpsim r g R RR ps pt nths (st_s, trigger (Choose X) >>= k_s) (st_t, i_t) E.
   Proof.
     unseal; iIntros "[%x RR] I". iApply isim_choose_src; eauto. iExists _; iApply "RR"; iFrame.
   Qed.
 
-  Lemma wpsim_choose_tgt X r g R RR ps pt nths st_s st_t i_s k_t u n E :
-    (∀ x, wpsim r g R RR ps true nths (st_s, i_s) (st_t, k_t x) u n E) ⊢
-    wpsim r g R RR ps pt nths (st_s, i_s) (st_t, trigger (Choose X) >>= k_t) u n E.
+  Lemma wpsim_choose_tgt X r g R RR ps pt nths st_s st_t i_s k_t E :
+    (∀ x, wpsim r g R RR ps true nths (st_s, i_s) (st_t, k_t x) E) ⊢
+    wpsim r g R RR ps pt nths (st_s, i_s) (st_t, trigger (Choose X) >>= k_t) E.
   Proof.
     unseal; iIntros "RR I". iApply isim_choose_tgt; eauto. iIntros (x); iApply "RR"; iFrame.
   Qed.
 
-  Lemma wpsim_sput_src k v r g R RR ps pt nths st_s st_t k_s i_t u n E :
-    wpsim r g R RR true pt nths (alist_upd k v st_s, k_s tt) (st_t, i_t) u n E ⊢
-    wpsim r g R RR ps pt nths (st_s, trigger (SPut k v) >>= k_s) (st_t, i_t) u n E.
+  Lemma wpsim_sput_src k v r g R RR ps pt nths st_s st_t k_s i_t E :
+    wpsim r g R RR true pt nths (alist_upd k v st_s, k_s tt) (st_t, i_t) E ⊢
+    wpsim r g R RR ps pt nths (st_s, trigger (SPut k v) >>= k_s) (st_t, i_t) E.
   Proof. unseal; iIntros "RR I". iApply isim_sput_src; eauto. iApply "RR"; iFrame. Qed.
 
-  Lemma wpsim_sput_tgt k v r g R RR ps pt nths st_s st_t i_s k_t u n E :
-    wpsim r g R RR ps true nths (st_s, i_s) (alist_upd k v st_t, k_t tt) u n E ⊢
-    wpsim r g R RR ps pt nths (st_s, i_s) (st_t, trigger (SPut k v) >>= k_t) u n E.
+  Lemma wpsim_sput_tgt k v r g R RR ps pt nths st_s st_t i_s k_t E :
+    wpsim r g R RR ps true nths (st_s, i_s) (alist_upd k v st_t, k_t tt) E ⊢
+    wpsim r g R RR ps pt nths (st_s, i_s) (st_t, trigger (SPut k v) >>= k_t) E.
   Proof. unseal; iIntros "RR I". iApply isim_sput_tgt; eauto. iApply "RR"; iFrame. Qed.
 
-  Lemma wpsim_sget_src k r g R RR ps pt nths st_s st_t k_s i_t u n E :
-    wpsim r g R RR true pt nths (st_s, k_s (or_else (alist_find k st_s) tt↑)) (st_t, i_t) u n E ⊢
-    wpsim r g R RR ps pt nths (st_s, trigger (SGet k) >>= k_s) (st_t, i_t) u n E.
+  Lemma wpsim_sget_src k r g R RR ps pt nths st_s st_t k_s i_t E :
+    wpsim r g R RR true pt nths (st_s, k_s (or_else (alist_find k st_s) tt↑)) (st_t, i_t) E ⊢
+    wpsim r g R RR ps pt nths (st_s, trigger (SGet k) >>= k_s) (st_t, i_t) E.
   Proof. unseal; iIntros "RR I". iApply isim_sget_src; eauto. iApply "RR"; iFrame. Qed.
 
-  Lemma wpsim_sget_tgt k r g R RR ps pt nths st_s st_t i_s k_t u n E :
-    wpsim r g R RR ps true nths (st_s, i_s) (st_t, k_t (or_else (alist_find k st_t) tt↑)) u n E ⊢
-    wpsim r g R RR ps pt nths (st_s, i_s) (st_t, trigger (SGet k) >>= k_t) u n E.
+  Lemma wpsim_sget_tgt k r g R RR ps pt nths st_s st_t i_s k_t E :
+    wpsim r g R RR ps true nths (st_s, i_s) (st_t, k_t (or_else (alist_find k st_t) tt↑)) E ⊢
+    wpsim r g R RR ps pt nths (st_s, i_s) (st_t, trigger (SGet k) >>= k_t) E.
   Proof. unseal; iIntros "RR I". iApply isim_sget_tgt; eauto. iApply "RR"; iFrame. Qed.
 
-  Lemma wpsim_assume_src (P : iProp Σ) r g R RR ps pt nths st_s st_t k_s i_t u n E :
-    (P -∗ wpsim r g R RR true pt nths (st_s, k_s tt) (st_t, i_t) u n E) ⊢
-    wpsim r g R RR ps pt nths (st_s, trigger (Assume P) >>= k_s) (st_t, i_t) u n E.
+  Lemma wpsim_assume_src (P : iProp Σ) r g R RR ps pt nths st_s st_t k_s i_t E :
+    (P -∗ wpsim r g R RR true pt nths (st_s, k_s tt) (st_t, i_t) E) ⊢
+    wpsim r g R RR ps pt nths (st_s, trigger (Assume P) >>= k_s) (st_t, i_t) E.
   Proof.
     unseal; iIntros "RR I". iApply isim_Assume_src; eauto. iIntros "P".
     iApply ("RR" with "P"); iFrame.
   Qed.
 
-  Lemma wpsim_assume_tgt (P : iProp Σ) r g R RR ps pt nths st_s st_t i_s k_t u n E :
-    P ∗ wpsim r g R RR ps true nths (st_s, i_s) (st_t, k_t tt) u n E ⊢
-    wpsim r g R RR ps pt nths (st_s, i_s) (st_t, trigger (Assume P) >>= k_t) u n E.
+  Lemma wpsim_assume_tgt (P : iProp Σ) r g R RR ps pt nths st_s st_t i_s k_t E :
+    P ∗ wpsim r g R RR ps true nths (st_s, i_s) (st_t, k_t tt) E ⊢
+    wpsim r g R RR ps pt nths (st_s, i_s) (st_t, trigger (Assume P) >>= k_t) E.
   Proof. unseal; iIntros "[P RR] I". iApply isim_Assume_tgt; eauto. iFrame. iApply "RR". ss. Qed.
 
-  Lemma wpsim_guarantee_src (P : iProp Σ) r g R RR ps pt nths st_s st_t k_s i_t u n E :
-    P ∗ wpsim r g R RR true pt nths (st_s, k_s tt) (st_t, i_t) u n E ⊢
-    wpsim r g R RR ps pt nths (st_s, trigger (Guarantee P) >>= k_s) (st_t, i_t) u n E.
+  Lemma wpsim_guarantee_src (P : iProp Σ) r g R RR ps pt nths st_s st_t k_s i_t E :
+    P ∗ wpsim r g R RR true pt nths (st_s, k_s tt) (st_t, i_t) E ⊢
+    wpsim r g R RR ps pt nths (st_s, trigger (Guarantee P) >>= k_s) (st_t, i_t) E.
   Proof. unseal; iIntros "[P RR] I". iApply isim_Guarantee_src; eauto. iFrame. iApply "RR"; ss. Qed.
 
-  Lemma wpsim_guarantee_tgt (P : iProp Σ) r g R RR ps pt nths st_s st_t i_s k_t u n E :
-    P ∗ wpsim r g R RR ps true nths (st_s, i_s) (st_t, k_t tt) u n E ⊢
-    wpsim r g R RR ps pt nths (st_s, i_s) (st_t, trigger (Assume P) >>= k_t) u n E.
+  Lemma wpsim_guarantee_tgt (P : iProp Σ) r g R RR ps pt nths st_s st_t i_s k_t E :
+    P ∗ wpsim r g R RR ps true nths (st_s, i_s) (st_t, k_t tt) E ⊢
+    wpsim r g R RR ps pt nths (st_s, i_s) (st_t, trigger (Assume P) >>= k_t) E.
   Proof. unseal; iIntros "[P RR] I". iApply isim_Assume_tgt; eauto. iFrame. iApply "RR". ss. Qed.
+
+  Lemma wpsim_spawn r g R RR ps pt nths st_s st_t fn args k_s k_t E :
+    wpsim r g R RR true true (S nths) (st_s, k_s nths) (st_t, k_t nths) E ⊢
+    wpsim r g R RR ps pt nths
+      (st_s, trigger (Spawn fn args) >>= k_s)
+      (st_t, trigger (Spawn fn args) >>= k_t) E.
+  Proof. unseal; iIntros "C I". iApply isim_spawn; eauto. iApply "C". ss. Qed.
+
+  Lemma wpsim_yield r g R RR ps pt nths st_s st_t tid k_s k_t E :
+    Ist nths st_s st_t ∗
+    (∀ nths' st_s' st_t' (NODS : List.NoDup (map fst st_s')) (NODT : List.NoDup (map fst st_t')),
+      Ist nths' st_s' st_t' -∗
+      wpsim r g R RR true true nths' (st_s', k_s tt) (st_t', k_t tt) E) ⊢
+    wpsim r g R RR ps pt nths
+      (st_s, trigger (Yield tid) >>= k_s)
+      (st_t, trigger (Yield tid) >>= k_t) E.
+  Proof.
+    unseal; iIntros "[IST C] I". iApply isim_yield; eauto. iFrame.
+    iIntros (?????) "IST"; iApply ("C" with "[] [] [IST] [I]"); iFrame; iPureIntro; ss.
+  Qed.
+
+  Lemma wpsim_tid_src r g R RR ps pt nths st_s st_t k_s i_t E :
+    wpsim r g R RR true pt nths (st_s, k_s my_tid) (st_t, i_t) E ⊢
+    wpsim r g R RR ps pt nths (st_s, trigger Tid >>= k_s) (st_t, i_t) E.
+  Proof. unseal; iIntros "RR I". iApply isim_tid_src; iApply "RR"; iFrame. Qed.
+
+  Lemma wpsim_tid_tgt r g R RR ps pt nths st_s st_t i_s k_t E :
+    wpsim r g R RR ps true nths (st_s, i_s) (st_t, k_t my_tid) E ⊢
+    wpsim r g R RR ps pt nths (st_s, i_s) (st_t, trigger Tid >>= k_t) E.
+  Proof. unseal; iIntros "RR I". iApply isim_tid_tgt; iApply "RR"; iFrame. Qed.
+
+  Lemma wpsim_progress r g R RR nths st_s st_t i_s i_t E :
+    wpsim g g R RR false false nths (st_s, i_s) (st_t, i_t) E ⊢
+    wpsim r g R RR true true nths (st_s, i_s) (st_t, i_t) E.
+  Proof. unseal; iIntros "RR I". iApply isim_progress; iApply "RR"; iFrame. Qed.
+
+  Lemma wpsim_base r g R RR ps pt nths st_s st_t i_s i_t :
+    r R RR ps pt nths (st_s, i_s) (st_t, i_t) ⊢
+    wpsim r g R RR ps pt nths (st_s, i_s) (st_t, i_t) ⊤.
+  Proof. unseal; iIntros "RR I". iApply isim_base; iFrame. Qed.
+
+  Lemma wpsim_coind (r g : rel) A P RA RRA psA ptA nthsA srcA tgtA :
+    (∀ (g' : rel) (a : A),
+      P a -∗
+      (□ ∀ R RR ps pt nths0 src tgt, g R RR ps pt nths0 src tgt -∗ g' R RR ps pt nths0 src tgt) -∗
+      (□ ∀ a, P a -∗ g' (RA a) (RRA a) (psA a) (ptA a) (nthsA a) (srcA a) (tgtA a)) -∗
+      wpsim r g' (RA a) (RRA a) (psA a) (ptA a) (nthsA a) (srcA a) (tgtA a) ⊤) →
+    ∀ (a : A), P a ⊢ wpsim r g (RA a) (RRA a) (psA a) (ptA a) (nthsA a) (srcA a) (tgtA a) ⊤.
+  Proof.
+    unseal; intros H a; iIntros "P I"; iCombine "P I" as "P". iStopProof.
+    revert a. eapply isim_coind.
+    intros g' a Himpl; iIntros "[[P I] #CIH]".
+    iPoseProof (H with "P [] [] I") as "H".
+    { instantiate (1 :=
+        (λ R RR ps pt nths '(st_s, i_s) '(st_t, i_t),
+          wpsim_pre ⊤ -∗ g' R RR ps pt nths (st_s, i_s) (st_t, i_t))%I).
+      iModIntro; iIntros (???????) "G"; destruct src, tgt; iIntros "I". iApply Himpl; iFrame.
+    }
+    { iModIntro; iIntros (a') "P"; iSpecialize ("CIH" $! a'); destruct (srcA a'), (tgtA a').
+      iIntros "I"; iApply "CIH"; iFrame.
+    }
+    iApply (isim_mono_knowledge with "H"); ss.
+    { iIntros (???????) "H"; iModIntro; iFrame. }
+    { iIntros (???????) "H !>"; destruct sti_src, sti_tgt; rewrite /wpsim_rel.
+      iDestruct "H" as "[H1 H2]"; iApply "H2"; iFrame.
+    }
+  Qed.
 End wpsim.
 (* TODO : proofmode instances *)
